ConstrainedDecodingFormalization/RealizableSequence.lean
@@ -1,7 +1,7 @@
 import ConstrainedDecodingFormalization.Automata
-import ConstrainedDecodingFormalization.Vocabulary
 import ConstrainedDecodingFormalization.Lexing
 import ConstrainedDecodingFormalization.RegularExpressionsToEpsilonNFA
+import Mathlib.Data.FinEnum
 import Mathlib.Computability.NFA
 import Mathlib.Computability.DFA
 import Mathlib.Computability.RegularExpressions
@@ -16,7 +16,6 @@ open Classical List RegularExpression
 universe u v w x
 variable {α : Type u} {Γ : Type v} { V : Type x } { σ0 σ1 σ2 : Type w}
 
-abbrev Vocab (α : Type u) := List (Token α Γ)
 abbrev State (α : Type u) := List α
 abbrev Next (α : Type u) := List (State α)
 abbrev Output (α : Type u):= List (List α)
@@ -28,15 +27,13 @@ namespace Detokenizing
 
 variable [BEq V]
 
-def BuildDetokenizingFST (tokens: List (Token α V)): FST V α Nat :=
-  let states := [0]
+def BuildDetokenizingFST (tokens: List (Token α V)): FST V α Unit :=
   let step := fun _ s =>
     match tokens.find? λ t => t.symbol == s with
-    | some t => (0, t.string)
+    | some t => (Unit.unit, t.string)
     | none => none
 
-  let alph := tokens.map (fun t => t.symbol)
-  FST.mk alph.eraseDups states 0 step [0]
+  FST.mk Unit.unit step [Unit.unit]
 
 def detokenize (tokens: List (Token α V)) (w : List V) : Option (List α) :=
   match w with
@@ -51,7 +48,7 @@ def detokenize (tokens: List (Token α V)) (w : List V) : Option (List α) :=
 theorem detokenizerFST_eq_detokenizer  ( tokens : List (Token α V)) :
   ∀ ( w : List V ), detokenize tokens w = ((BuildDetokenizingFST tokens).eval w).map Prod.snd := by
   intro w
-  have lem : ∀ w, detokenize tokens w = ((BuildDetokenizingFST tokens).evalFrom 0 w).map Prod.snd := by
+  have lem : ∀ w, detokenize tokens w = ((BuildDetokenizingFST tokens).evalFrom Unit.unit w).map Prod.snd := by
     intro w
     induction w
     case nil =>
@@ -107,29 +104,16 @@ variable
   [Inhabited α] [Inhabited Γ]
   [Fintype α] [Fintype Γ]
 
-#check Vocabulary (Ch α) (Γ)
-
---def VocabStr [Vocabulary (Ch α) (Γ)] (x : V) : List (Ch α) :=
- -- sorry
-
 #check Language (Ch α)
 
-
-noncomputable def characterAlphabetSet (α : Type u) [Fintype (Ch α)] : List (Ch α) :=
-  (Finset.univ : Finset (Ch α)).toList
-
-noncomputable def BuildTokenLevelFST (fst_lex : FSTLex α Γ σ0) (fst_detok : FSTDetok α σ1) :
-    FST (Token (Ch α)) Γ (σ0 × σ1) := Id.run do
-  sorry
-
-def RealizableSequences (fst_comp : FSTComp α Γ σ2) : Set (List Γ) :=
+def RealizableSequences (fst_comp : FST α Γ σ2) : Set (List Γ) :=
   -- all possible transitions, adjoined with singleton transitions afterwards
   { Ts' | ∃ q_0 t Ts q_1 T,
           fst_comp.step q_0 t = some (q_1, Ts) ∧
           T ∈ fst_comp.singleProducible q_1 ∧
           Ts' = Ts ++ [T] }
 
-def InverseTokenSpannerTable (fst_comp : FSTComp α Γ σ2) : List Γ → σ2 → (Set (Token (Ch α))) :=
+def InverseTokenSpannerTable (fst_comp : FST α Γ σ2) : List Γ → σ2 → (Set α) :=
   fun rs st =>
     if h : rs ≠ [] then
       let Ts := rs.dropLast
@@ -139,15 +123,45 @@ def InverseTokenSpannerTable (fst_comp : FSTComp α Γ σ2) : List Γ → σ2 �
             T ∈ fst_comp.singleProducible q_1 }
     else ∅
 
-def BuildInverseTokenSpannerTable (fst_comp : FSTComp α Γ σ2) : Re Γ × (List Γ → σ2 → (List (Token (Ch α)))) := Id.run do
-  sorry
 
-def itst_fst_eq_rs (fst_comp : FSTComp α Γ σ2) : (BuildInverseTokenSpannerTable fst_comp).fst.toFinset = RealizableSequences fst_comp := by sorry
+variable [ q: FinEnum σ2 ] [ a: FinEnum α ] [ t: FinEnum Γ ]
 
-def itst_snd_eq_itst (fst_comp : FSTComp α Γ σ2) :
+def BuildInverseTokenSpannerTable
+  (fst_comp : FST α Γ σ2) : Re Γ × (List Γ → σ2 → (List α)) := Id.run do
+  let Q := q.toList
+  let A := a.toList
+
+  let re :=
+    Q.flatMap (fun q =>
+      A.flatMap ( fun c =>
+        match fst_comp.step q c with
+        | none => []
+        | some (q', Ts) =>
+          (fst_comp.computeSingleProducible q')
+          |>.map (fun t => Ts ++ [t])
+      )
+    )
+    |>.eraseDups
+
+  let tinv := fun rs s =>
+    if h : rs ≠ [] then
+      let Ts := rs.dropLast
+      let T := rs.getLast h
+      A.filter (fun c =>
+        match fst_comp.step s c with
+        | none => false
+        | some (q', Ts') => (fst_comp.computeSingleProducible q').contains T && Ts' = Ts
+      )
+    else []
+
+  (re, tinv)
+
+def itst_fst_eq_rs (fst_comp : FST α Γ σ2) : (BuildInverseTokenSpannerTable fst_comp).fst.toFinset = RealizableSequences fst_comp := by sorry
+
+def itst_snd_eq_itst (fst_comp : FST α Γ σ2) :
     ∀ rs s, ((BuildInverseTokenSpannerTable fst_comp).snd rs s).toFinset = InverseTokenSpannerTable fst_comp rs s := by sorry
 
 end Symbols
 
-theorem rs_ne_empty (fst_comp : FSTComp α Γ σ2) : [] ∉ RealizableSequences fst_comp := by
+theorem rs_ne_empty (fst_comp : FST α Γ σ2) : [] ∉ RealizableSequences fst_comp := by
   simp_all[RealizableSequences]
